+++
title = "Sine Law"
date = 2022-01-04T11:11:56-05:00
draft = false

unit = 7
lesson = 1
chapter = 8
section = 1
+++

The sine law is as follows:
{{<mi>}}\frac{a}{\sin{A}} \,=\, \frac{b}{\sin{B}} \,=\, \frac{c}{\sin{C}} \,=\, 2R{{</mi>}},
where
{{<mi>}}a{{</mi>}},
{{<mi>}}b{{</mi>}}, and
{{<mi>}}c{{</mi>}},
are the lengths of the sides of the triangle, and
{{<mi>}}\alpha{{</mi>}},
{{<mi>}}\beta{{</mi>}}, and
{{<mi>}}\gamma{{</mi>}},
are the opposite angles of the sides, and
{{<mi>}}R{{</mi>}} is the radius of the triangle's circumcircle.

The sine law can be used to find the other sides of an acute triangle when two angles and a side are given.

Here is a figure that shows the relationship graphically.
{{<cite/wmc "File:Law_of_sines_in_plane_trigonometry-20201220.svg">}}

The proof is as follows:

Assume a triangle {{<mi>}}\triangle ABC{{</mi>}},
where,
{{<mi>}}h{{</mi>}} is a line
from {{<mi>}}A{{</mi>}}
to {{<mi>}}D{{</mi>}} (which is a point on {{<mi>}}\overline{BC}{{</mi>}})
where,
{{<mi>}}\angle ADC=\angle ADB=90^{\circ}{{</mi>}}.

Using the definiton of the sine function,
{{<mi>}}sinB=\frac{h}{c}{{</mi>}}, and
{{<mi>}}sinC=\frac{h}{b}{{</mi>}}.

They can be rewritten as
{{<mi>}}h=csinB{{</mi>}}, and
{{<mi>}}h=bsinC{{</mi>}}, or
{{<mi>}}csinB=bsinC{{</mi>}}.

Therefore, {{<mi>}}\frac{c}{sinC}=\frac{b}{sinB}{{</mi>}}.

Repeating the above on
line {{<mi>}}j{{</mi>}},
which goes
from {{<mi>}}b{{</mi>}}
to {{<mi>}}E{{</mi>}} (whcih is a point on {{<mi>}}\overline{AC}{{</mi>}})
where,
{{<mi>}}\angle BEA=\angle BEC=90^{\circ}{{</mi>}},
yields
{{<mi>}}\frac{c}{sinC}=\frac{a}{sinA}{{</mi>}}.
